@prefix IAO: <http://purl.obolibrary.org/obo/IAO_> .
@prefix RO: <http://purl.obolibrary.org/obo/RO_> .
@prefix dcterms: <http://purl.org/dc/terms/> .
@prefix linkml: <https://w3id.org/linkml/> .
@prefix owl: <http://www.w3.org/2002/07/owl#> .
@prefix rdf: <http://www.w3.org/1999/02/22-rdf-syntax-ns#> .
@prefix rdfs: <http://www.w3.org/2000/01/rdf-schema#> .
@prefix skos: <http://www.w3.org/2004/02/skos/core#> .
@prefix tc: <https://w3id.org/linkml/taxon_constraints/> .
@prefix xsd: <http://www.w3.org/2001/XMLSchema#> .

linkml:taxon_constraints.owl.ttl a owl:Ontology ;
    rdfs:label "taxon-constraints" ;
    IAO:0000700 tc:TaxonConstraint,
        tc:Term ;
    dcterms:license "https://creativecommons.org/publicdomain/zero/1.0/" ;
    dcterms:title "Taxon Constraints Reporting Datamodel" ;
    linkml:generation_date "2023-02-27T09:54:53" ;
    linkml:metamodel_version "1.7.0" ;
    linkml:source_file "taxon_constraints.yaml" ;
    linkml:source_file_date "2023-02-21T13:39:48" ;
    linkml:source_file_size 5692 .

tc:asserted a owl:DatatypeProperty ;
    rdfs:label "asserted" ;
    rdfs:range xsd:boolean ;
    skos:definition "holds if the constraint is asserted in the source ontology, rather than inferred by rules or reasoning" .

tc:candidate a owl:DatatypeProperty ;
    rdfs:label "candidate" ;
    rdfs:range xsd:boolean ;
    skos:definition "true if this is a proposed candidate constraint" .

tc:comments a owl:DatatypeProperty ;
    rdfs:label "comments" ;
    rdfs:range xsd:string .

tc:contradicted_by a owl:ObjectProperty ;
    rdfs:label "contradicted_by" ;
    rdfs:range tc:TaxonConstraint ;
    skos:definition "If the taxon constraint conflicts with another,  then this is the set of taxon constraints that it is redundant with" .

tc:description a owl:DatatypeProperty ;
    rdfs:label "description" ;
    rdfs:range xsd:string ;
    skos:definition "A description of the term" .

tc:evolutionary a owl:DatatypeProperty ;
    rdfs:label "evolutionary" ;
    rdfs:range xsd:boolean ;
    skos:definition "holds if the constraint is an evolutionary statement" .

tc:id a owl:DatatypeProperty ;
    rdfs:label "id" ;
    rdfs:range xsd:anyURI ;
    skos:definition "the OBO CURIE for the term" .

tc:predicates a owl:ObjectProperty ;
    rdfs:label "predicates" ;
    rdfs:range tc:PredicateTerm ;
    skos:definition "The predicates that connect the subject term to the via_terms." .

tc:present_in_ancestor_of a owl:ObjectProperty ;
    rdfs:label "present_in_ancestor_of" ;
    rdfs:range tc:TaxonConstraint .

tc:redundant a owl:DatatypeProperty ;
    rdfs:label "redundant" ;
    rdfs:range xsd:boolean ;
    skos:definition "True if this is redundant within the set of constraints of the same type (never vs only)" .

tc:redundant_with a owl:ObjectProperty ;
    rdfs:label "redundant_with" ;
    rdfs:range tc:TaxonConstraint ;
    skos:definition "If the taxon constraint is redundant, then this is the set of taxon constraints that it is redundant with" .

tc:redundant_with_only_in a owl:DatatypeProperty ;
    rdfs:label "redundant_with_only_in" ;
    rdfs:range xsd:boolean ;
    skos:definition "True for never in constraints that are subsumed by an only in" .

tc:sources a owl:DatatypeProperty ;
    rdfs:label "sources" ;
    rdfs:range xsd:anyURI .

tc:unsatisfiable a owl:DatatypeProperty ;
    rdfs:label "unsatisfiable" ;
    rdfs:range xsd:boolean ;
    skos:definition "If true then some combination of taxon constraints plus ontology lead to contradictions" .

tc:via_terms a owl:ObjectProperty ;
    rdfs:label "via_terms" ;
    rdfs:range tc:SubjectTerm ;
    skos:definition "For inferred taxon constraints, this is the term or terms that have the taxon constraint asserted" .

RO:0002160 a owl:ObjectProperty ;
    rdfs:label "only_in" ;
    rdfs:range tc:TaxonConstraint ;
    skos:definition """Points to a taxon constraint that states the SubjectTerm is ONLY found in a taxon or descendant. Formally, the term AND its descendants MUST be in the specified taxon, or a descendant of that taxon
""" ;
    skos:exactMatch RO:0002160 ;
    skos:note "Note that we conflate between the RO \"only in taxon\" and \"in taxon\" relations here" .

RO:0002161 a owl:ObjectProperty ;
    rdfs:label "never_in" ;
    rdfs:range tc:TaxonConstraint ;
    skos:definition """Points to a taxon constraint that states the SubjectTerm is NEVER found in a taxon or descendant. Formally, the term AND its descendants MUST NOT be in the specified taxon, or a descendant of that taxon
""" ;
    skos:exactMatch RO:0002161 .

RO:0002175 a owl:ObjectProperty ;
    rdfs:label "present_in" ;
    rdfs:range tc:TaxonConstraint ;
    skos:definition """The term MAY be in the specified taxon, or a descendant of that taxon
""" ;
    skos:exactMatch RO:0002175 .

rdf:object a owl:ObjectProperty ;
    rdfs:label "taxon" ;
    rdfs:range tc:Taxon ;
    skos:definition "The taxon which this constraint is about. May be species or a more general class." ;
    skos:exactMatch rdf:object .

rdf:predicate a owl:ObjectProperty ;
    rdfs:label "predicate" ;
    rdfs:range tc:PredicateTerm ;
    skos:definition "The relationship type for the contraint (e.g. in_taxon, never_in taxon)" ;
    skos:exactMatch rdf:predicate .

rdf:subject a owl:ObjectProperty ;
    rdfs:label "subject" ;
    rdfs:range tc:SubjectTerm ;
    skos:definition "The term to which the constraint applies" ;
    skos:exactMatch rdf:subject ;
    skos:note "this is a reciprocal slot and will be the same as the containing SubjectTerm" .

rdfs:label a owl:DatatypeProperty ;
    rdfs:label "label" ;
    rdfs:range xsd:string ;
    skos:definition "the human readable name or label of the term" ;
    skos:exactMatch rdfs:label .

tc:Taxon a owl:Class ;
    rdfs:label "Taxon" ;
    rdfs:subClassOf tc:Term ;
    skos:definition "A term that represents a taxonomic group, may be at species level of a higher level" ;
    skos:exactMatch <http://example.org/UNKNOWN/NCBITaxon/1> .

tc:PredicateTerm a owl:Class ;
    rdfs:label "PredicateTerm" ;
    rdfs:subClassOf tc:Term ;
    skos:definition "A term that represents a relationship type" .

tc:SubjectTerm a owl:Class ;
    rdfs:label "SubjectTerm" ;
    rdfs:subClassOf [ a owl:Restriction ;
            owl:allValuesFrom tc:TaxonConstraint ;
            owl:onProperty RO:0002161 ],
        [ a owl:Restriction ;
            owl:allValuesFrom tc:TaxonConstraint ;
            owl:onProperty tc:present_in_ancestor_of ],
        [ a owl:Restriction ;
            owl:maxQualifiedCardinality 1 ;
            owl:onDataRange xsd:boolean ;
            owl:onProperty tc:unsatisfiable ],
        [ a owl:Restriction ;
            owl:allValuesFrom tc:TaxonConstraint ;
            owl:onProperty RO:0002175 ],
        [ a owl:Restriction ;
            owl:maxQualifiedCardinality 1 ;
            owl:onDataRange xsd:string ;
            owl:onProperty tc:description ],
        [ a owl:Restriction ;
            owl:allValuesFrom tc:TaxonConstraint ;
            owl:onProperty RO:0002160 ],
        tc:Term ;
    skos:definition "A term that is the subject of a taxon constraint. Typically comes from ontologies like GO, UBERON, CL, ..." .

tc:Term a owl:Class ;
    rdfs:label "Term" ;
    rdfs:subClassOf [ a owl:Restriction ;
            owl:maxQualifiedCardinality 1 ;
            owl:onDataRange xsd:string ;
            owl:onProperty rdfs:label ],
        [ a owl:Restriction ;
            owl:onDataRange xsd:anyURI ;
            owl:onProperty tc:id ;
            owl:qualifiedCardinality 1 ] ;
    skos:definition "An ontology term. In this model this is either the SubjectTerm of a taxon constraint, or an actual taxon" ;
    skos:exactMatch owl:Class .

tc:TaxonConstraint a owl:Class ;
    rdfs:label "TaxonConstraint" ;
    rdfs:subClassOf [ a owl:Restriction ;
            owl:maxQualifiedCardinality 1 ;
            owl:onClass tc:PredicateTerm ;
            owl:onProperty rdf:predicate ],
        [ a owl:Restriction ;
            owl:maxQualifiedCardinality 1 ;
            owl:onClass tc:Taxon ;
            owl:onProperty rdf:object ],
        [ a owl:Restriction ;
            owl:maxQualifiedCardinality 1 ;
            owl:onDataRange xsd:boolean ;
            owl:onProperty tc:redundant_with_only_in ],
        [ a owl:Restriction ;
            owl:maxQualifiedCardinality 1 ;
            owl:onDataRange xsd:boolean ;
            owl:onProperty tc:redundant ],
        [ a owl:Restriction ;
            owl:allValuesFrom tc:PredicateTerm ;
            owl:onProperty tc:predicates ],
        [ a owl:Restriction ;
            owl:maxQualifiedCardinality 1 ;
            owl:onDataRange xsd:boolean ;
            owl:onProperty tc:asserted ],
        [ a owl:Restriction ;
            owl:allValuesFrom tc:SubjectTerm ;
            owl:onProperty tc:via_terms ],
        [ a owl:Restriction ;
            owl:allValuesFrom xsd:anyURI ;
            owl:onProperty tc:sources ],
        [ a owl:Restriction ;
            owl:maxQualifiedCardinality 1 ;
            owl:onDataRange xsd:boolean ;
            owl:onProperty tc:candidate ],
        [ a owl:Restriction ;
            owl:allValuesFrom tc:TaxonConstraint ;
            owl:onProperty tc:contradicted_by ],
        [ a owl:Restriction ;
            owl:allValuesFrom tc:TaxonConstraint ;
            owl:onProperty tc:redundant_with ],
        [ a owl:Restriction ;
            owl:maxQualifiedCardinality 1 ;
            owl:onClass tc:SubjectTerm ;
            owl:onProperty rdf:subject ],
        [ a owl:Restriction ;
            owl:allValuesFrom xsd:string ;
            owl:onProperty tc:comments ],
        [ a owl:Restriction ;
            owl:maxQualifiedCardinality 1 ;
            owl:onDataRange xsd:boolean ;
            owl:onProperty tc:evolutionary ] ;
    skos:definition "An individual taxon constraint" ;
    skos:exactMatch rdf:Statement .



